Use Typeclasses

doc/coq/Abstract.v
@@ -1,124 +1,34 @@
 From MODULAR Require Export Syntax.
 
-Definition time := bool.
+Generalizable Variables T.
 
-Definition path := list time.
-
-Definition eq_t (t1 t2 : time) := Bool.eqb t1 t2.
-
-Fixpoint eq_p (p1 p2 : path) :=
-  match p1, p2 with
-  | [], [] => true
-  | hd1 :: tl1, [] => false
-  | [], hd2 :: tl2 => false
-  | hd1 :: tl1, hd2 :: tl2 =>
-    if eq_t hd1 hd2 then eq_p tl1 tl2
-                    else false
-  end.
-
-Definition len_p (p : path) := List.length p.
-
-Lemma eq_t_eq :
-  forall t1 t2, eq_t t1 t2 = true <-> t1 = t2.
-Proof.
-  unfold eq_t. apply Bool.eqb_true_iff.
-Qed.
-
-Lemma eq_t_neq :
-  forall t1 t2, eq_t t1 t2 = false <-> t1 <> t2.
-Proof.
-  unfold eq_t. apply Bool.eqb_false_iff.
-Qed.
-
-Inductive dy_ctx :=
-  | dy_c_hole
-  | dy_c_lam (x: expr_id) (tx : time) (C : dy_ctx)
-  | dy_c_lete (x : expr_id) (tx : time) (C : dy_ctx)
-  | dy_c_letm (M : mod_id) (CM : dy_ctx) (C : dy_ctx)
-.
-
-Fixpoint dy_plugin_c Cout Cin :=
-  match Cout with
-  | dy_c_hole => Cin
-  | dy_c_lam x tx C' => dy_c_lam x tx (dy_plugin_c C' Cin)
-  | dy_c_lete x tx C' => dy_c_lete x tx (dy_plugin_c C' Cin)
-  | dy_c_letm M CM C' => dy_c_letm M CM (dy_plugin_c C' Cin)
-  end.
-
-Fixpoint dy_level (C : dy_ctx) : path :=
-  match C with
-  | dy_c_hole => []
-  | dy_c_lam _ t C'
-  | dy_c_lete _ t  C' => dy_level C' ++ [t]
-  | dy_c_letm _ _  C' => dy_level C'
-  end.
-
-Fixpoint addr_x (C : dy_ctx) (x : expr_id) :=
-  match C with
-  | dy_c_hole => []
-  | dy_c_lam x' tx' C'
-  | dy_c_lete x' tx' C' =>
-    match addr_x C' x with
-    | [] => if eq_eid x x' then [tx'] else []
-    | addr => addr ++ [tx']
-    end
-  | dy_c_letm _ _ C' => addr_x C' x
-  end.
-
-Fixpoint ctx_M (C : dy_ctx) (M : mod_id) :=
-  match C with
-  | dy_c_hole => None
-  | dy_c_lam _ _ C'
-  | dy_c_lete _ _ C' => ctx_M C' M
-  | dy_c_letm M' CM' C' =>
-    match ctx_M C' M with
-    | Some CM => Some CM
-    | None => if eq_mid M M' then Some CM' else None
-    end
-  end.
-
-(* a term, a context *)
-Inductive expr_value :=
-  | Closure (x : expr_id) (e : tm) (C : dy_ctx)
-.
-
-Inductive dy_value :=
-  | EVal (ev : expr_value)
-  | MVal (mv : dy_ctx)
-.
-
-Inductive state :=
-  | ST (mem : path -> list expr_value)
+Inductive state {time : Type} :=
+  | ST (mem : time -> list (@expr_value time))
        (t : time)
 .
 
-Definition update_t (C : dy_ctx) (st : state) 
-                    (x : expr_id) (v : expr_value) :=
-  match st with
-  | ST mem t => negb t
-  end.
+Class Time `{OrderT T} :=
+{  
+  update : (@dy_ctx T) -> (@state T) -> expr_id -> (@expr_value T) -> T;
+}.
 
-Definition update_m {X} mem (p : path) (x : X) :=
-  fun p1 => 
-  if eq_p p1 p then
-    x :: (mem p)
-  else mem p1.
+Definition update_m {X} `{Time T} mem (t : T) (x : X) :=
+  fun t' => 
+  if eqb t' t then
+    x :: (mem t)
+  else mem t'.
 
-Definition empty_mem {X} (p : path) : list X := [].
+Definition empty_mem {X T} (t : T) : list X := [].
 
 Notation "p '!#->' v ';' mem" := (update_m mem p v)
                               (at level 100, v at next level, right associativity).
 
-Notation "Cout '[#|' Cin '|#]'" := (dy_plugin_c Cout Cin)
-                              (at level 100, Cin at next level, right associativity).
-Notation "'[#||#]'" := (dy_c_hole) (at level 100).
-
-Inductive EvalR (C : dy_ctx) (st : state)
+Inductive EvalR `{Time T} (C : @dy_ctx T) (st : @state T)
     : tm -> dy_value -> state -> Prop :=
-  | Eval_var_e x v mem t
+  | Eval_var_e x v mem t addr
              (STATE : ST mem t = st)
-             (ADDR : [] <> addr_x C x)
-             (ACCESS : In v (mem (addr_x C x)))
+             (ADDR : Some addr = addr_x C x)
+             (ACCESS : In v (mem addr))
     : EvalR C st (e_var x) (EVal v) st
   | Eval_lam x e
     : EvalR C st (e_lam x e)
@@ -131,9 +41,9 @@ Inductive EvalR (C : dy_ctx) (st : state)
                          (EVal (Closure x e C_lam)) st_lam)
              (ARG : EvalR C st_lam e2
                           (EVal arg) (ST mem t))
-             (BODY : EvalR (C_lam [#|dy_c_lam x t ([#||#])|#])
-                           (ST (t :: (dy_level C_lam) !#-> arg ; mem) 
-                               (update_t C (ST mem t) x arg))
+             (BODY : EvalR (C_lam [|dy_c_lam x t ([||])|])
+                           (ST (t !#-> arg ; mem) 
+                               (update C (ST mem t) x arg))
                            e (EVal v) st_v)
     : EvalR C st (e_app e1 e2) (EVal v) st_v
   | Eval_link m e C_m st_m v st_v
@@ -147,24 +57,24 @@ Inductive EvalR (C : dy_ctx) (st : state)
   | Eval_lete x e v mem t
               m C_m st_m
                (EVALe : EvalR C st e (EVal v) (ST mem t))
-               (EVALm : EvalR (C [#|dy_c_lete x t ([#||#])|#])
-                        (ST (t :: (dy_level C) !#-> v ; mem) 
-                            (update_t C (ST mem t) x v))
+               (EVALm : EvalR (C [|dy_c_lete x t ([||])|])
+                        (ST (t !#-> v ; mem) 
+                            (update C (ST mem t) x v))
                         m (MVal C_m) st_m)
     : EvalR C st (m_lete x e m) (MVal C_m) st_m
   | Eval_letm M m' C' st'
               m'' C'' st''
               (EVALm' : EvalR C st m' (MVal C') st')
-              (EVALm'' : EvalR (C [#|dy_c_letm M C' ([#||#])|#]) st'
+              (EVALm'' : EvalR (C [|dy_c_letm M C' ([||])|]) st'
                          m'' (MVal C'') st'')
     : EvalR C st (m_letm M m' m'') (MVal C'') st''
 .
 
-Definition Reach (tm1 tm2 : Type) := tm1 -> dy_ctx -> state -> tm2 -> Prop.
+#[export] Hint Constructors EvalR : core.
 
 (* Reachability relation *)
-Inductive ReachR (C : dy_ctx) (st : state)
-    : Reach tm tm :=
+Inductive ReachR `{Time T} (C : dy_ctx) (st : state)
+    : tm -> (@dy_ctx T) -> (@state T) -> tm -> Prop :=
   | r_refl e
     : ReachR C st e 
              C st e
@@ -187,9 +97,9 @@ Inductive ReachR (C : dy_ctx) (st : state)
                             (EVal (Closure x e C_lam)) st_lam)
                 (ARG : EvalR C st_lam e2
                              (EVal arg) (ST mem t))
-                (REACHb : ReachR (C_lam[#|dy_c_lam x t ([#||#])|#]) 
-                                 (ST (t :: (dy_level C_lam) !#-> arg ; mem) 
-                                     (update_t C (ST mem t) x arg)) e
+                (REACHb : ReachR (C_lam[|dy_c_lam x t ([||])|]) 
+                                 (ST (t !#-> arg ; mem) 
+                                     (update C (ST mem t) x arg)) e
                                  C' st' e')
     : ReachR C st (e_app e1 e2)
              C' st' e'
@@ -212,9 +122,9 @@ Inductive ReachR (C : dy_ctx) (st : state)
   | r_lete_m x e m v mem t
              C' st' e'
              (EVALx : EvalR C st e (EVal v) (ST mem t))
-             (REACHm : ReachR (C[#|dy_c_lete x t ([#||#])|#])
-                              (ST (t :: (dy_level C) !#-> v ; mem) 
-                                  (update_t C (ST mem t) x v)) m
+             (REACHm : ReachR (C[|dy_c_lete x t ([||])|])
+                              (ST (t !#-> v ; mem) 
+                                  (update C (ST mem t) x v)) m
                               C' st' e')
     : ReachR C st (m_lete x e m)
              C' st' e'
@@ -226,11 +136,13 @@ Inductive ReachR (C : dy_ctx) (st : state)
   | r_letm_m2 M m1 m2 C_M st_M
               C' st' e'
               (EVALM : EvalR C st m1 (MVal C_M) st_M)
-              (REACHm : ReachR (C[#|dy_c_letm M C_M ([#||#])|#]) st_M m2
+              (REACHm : ReachR (C[|dy_c_letm M C_M ([||])|]) st_M m2
                                C' st' e')
     : ReachR C st (m_letm M m1 m2)
              C' st' e'
 .
+
+#[export] Hint Constructors ReachR : core.
 
 Notation "'<|' C1 st1 tm1 '~#>' C2 st2 tm2 '|>'" := (ReachR C1 st1 tm1 C2 st2 tm2) 
                                                (at level 10, 
@@ -238,7 +150,7 @@ Notation "'<|' C1 st1 tm1 '~#>' C2 st2 tm2 '|>'" := (ReachR C1 st1 tm1 C2 st2 tm
                                                 C2 at next level, st2 at next level, tm2 at next level).
 
 (* sanity check *)
-Lemma reach_trans : forall C1 st1 e1
+Lemma reach_trans : forall `{Time T} (C1 : @dy_ctx T) st1 e1
                          C2 st2 e2
                          C3 st3 e3
                          (REACH1 : <| C1 st1 e1 ~#> C2 st2 e2 |>)
@@ -247,112 +159,21 @@ Lemma reach_trans : forall C1 st1 e1
 Proof.
   intros. generalize dependent e3.
   revert C3 st3.
-  induction REACH1; eauto using ReachR.
-Qed.
-
-Lemma c_plugin_assoc : forall C1 C2 C3, C1[#| C2[#| C3 |#] |#] = ((C1[#|C2|#])[#|C3|#]).
-Proof.
-  induction C1; eauto; 
-  intros; simpl; try rewrite IHC1; eauto.
-  rewrite IHC1_2. eauto.
-Qed.
-
-Lemma eq_p_eq : forall p1 p2, eq_p p1 p2 = true <-> p1 = p2.
-Proof.
-  induction p1; induction p2;
-  intros; simpl;
-  try rewrite IHp1; try rewrite IHp2;
-  eauto.
-  - split; eauto.
-  - split; intros contra; inversion contra.
-  - split; intros contra; inversion contra.
-  - simpl. remember (eq_t a a0) as eqa.
-    destruct eqa; symmetry in Heqeqa;
-    try rewrite eq_t_eq in Heqeqa;
-    try rewrite eq_t_neq in Heqeqa.
-    + split; intros. rewrite Heqeqa in *.
-      apply IHp1 in H. rewrite H. eauto.
-      eapply IHp1. inversion H; eauto.
-    + split; intros contra; inversion contra.
-      apply Heqeqa in H0; inversion H0.
-Qed.
-
-Lemma c_plugin_adds_level : forall C1 C2, eq_p (dy_level(C1 [#|C2|#] )) (dy_level C2 ++ dy_level C1) = true.
-Proof.
-  induction C1;
-  intros; try rewrite IHC1;
-  try apply Nat.eqb_eq; try rewrite app_nil_r in *; 
-  try rewrite c_plugin_assoc in *; simpl in *; 
-  eauto; try apply eq_p_eq; eauto;
-  specialize (IHC1 C2); rewrite eq_p_eq in IHC1;
-  rewrite IHC1; rewrite app_assoc; eauto.
-Qed.
-
-Fixpoint dy_to_st C :=
-  match C with
-  | ([#||#]) => st_c_hole
-  | dy_c_lam x _ C' => st_c_lam x (dy_to_st C')
-  | dy_c_lete x _ C' => st_c_lete x (dy_to_st C')
-  | dy_c_letm M CM C' => st_c_letm M (dy_to_st CM) (dy_to_st C')
-  end.
-
-Lemma dy_to_st_plugin :
-  forall Cout Cin,
-    dy_to_st (Cout[#|Cin|#]) = st_c_plugin (dy_to_st Cout) (dy_to_st Cin).
-Proof.
-  induction Cout; intros; simpl; try rewrite IHCout; eauto.
-  rewrite IHCout2. eauto.
-Qed. 
-
-Lemma mod_is_static_none : forall (dC : dy_ctx) (M : mod_id),
-  (ctx_M dC M = None <-> st_ctx_M (dy_to_st dC) M = None).
-Proof. 
-  intros. repeat split. 
-  - induction dC; simpl; eauto.
-    destruct (ctx_M dC2 M). intros H; inversion H.
-    specialize (IHdC2 eq_refl). rewrite IHdC2.
-    destruct (eq_mid M M0). intros H; inversion H. eauto.
-  - induction dC; simpl; eauto.
-    destruct (st_ctx_M (dy_to_st dC2) M). intros H; inversion H.
-    specialize (IHdC2 eq_refl). rewrite IHdC2.
-    destruct (eq_mid M M0). intros H; inversion H. eauto.
-Qed.
-
-Lemma mod_is_static_some : forall (dC : dy_ctx) (M : mod_id),
-  (forall v, ctx_M dC M = Some v -> st_ctx_M (dy_to_st dC) M = Some (dy_to_st v)) /\
-  (forall v, st_ctx_M (dy_to_st dC) M = Some v -> exists dv, dy_to_st dv = v /\ ctx_M dC M = Some dv).
-Proof.
-  intros; split. 
-  - induction dC; simpl; intros; eauto.
-    + inversion H.
-    + remember (ctx_M dC2 M) as v2. destruct v2.
-      specialize (IHdC2 v H). rewrite IHdC2. eauto.
-      symmetry in Heqv2. rewrite mod_is_static_none in Heqv2.
-      rewrite Heqv2. destruct (eq_mid M M0); inversion H; eauto.
-  - induction dC; simpl; intros; eauto.
-    + inversion H.
-    + remember (st_ctx_M (dy_to_st dC2) M) as v2. destruct v2.
-      specialize (IHdC2 v H). inversion IHdC2. exists x.
-      destruct H0. split. assumption. rewrite H1. eauto.
-      remember (ctx_M dC2 M) as v2. destruct v2;
-      symmetry in Heqv2; rewrite <- mod_is_static_none in Heqv2.
-      rewrite Heqv2 in Heqv0. inversion Heqv0.
-      destruct (eq_mid M M0). inversion H.
-      exists dC1. eauto. inversion H.
+  induction REACH1; eauto.
 Qed.
 
 Lemma value_reach_only_itself_e :
-  forall C st v (pf : value v)
+  forall `{Time T} (C : @dy_ctx T) st v (pf : value v)
          C' st' e'
          (REACH : <| C st v ~#> C' st' e' |>),
          C = C' /\ st = st' /\ v = e'.
 Proof.
-  intros; repeat split; inversion pf; inversion REACH; subst; eauto using ReachR;
-  try inversion H0.
+  intros; repeat split; inversion pf; inversion REACH; subst; eauto;
+  try inversion H2.
 Qed.
 
 Lemma Meval_then_collect :
-  forall C st m v st_m
+  forall `{Time T} C st m v st_m
          (EVAL : EvalR C st m v st_m)
          C_m (MVAL : v = MVal C_m),
         match collect_ctx (dy_to_st C) m with
@@ -360,7 +181,7 @@ Lemma Meval_then_collect :
         | (None, _) => False
         end.
 Proof.
-  intros. revert C_m MVAL.
+  intros. rename H into H'. rename H0 into H0'. revert C_m MVAL.
   induction EVAL; intros; simpl; try inversion MVAL; subst; eauto.
   - pose proof (mod_is_static_some C M) as H.
     destruct H as [A B]. specialize (A C_m).
@@ -378,7 +199,7 @@ Proof.
     apply IHEVAL2.
 Qed.
 
-Definition ctx_bound_st ub st:=
+Definition ctx_bound_st {T} ub (st : @state T) :=
   match st with
   | ST mem t =>
     forall addr x e C_v (INvl : In (Closure x e C_v) (mem addr))
@@ -386,15 +207,15 @@ Definition ctx_bound_st ub st:=
       In sC ub
   end.
 
-Definition ctx_bound_tm ub C st e :=
+Definition ctx_bound_tm {T} ub (C : @dy_ctx T) (st : @state T) e :=
   ctx_bound_st ub st /\
   let (o, ctxs) := collect_ctx (dy_to_st C) e in
   forall sC (IN : In sC ctxs),
          In sC ub.
 
 Lemma eval_ctx_bound :
-  forall ub
-         C st e
+  forall `{Time T} ub
+         (C : @dy_ctx T) st e
          v st'
          (INIT : ctx_bound_tm ub C st e)
          (EVAL : EvalR C st e v st'),
@@ -406,11 +227,11 @@ Lemma eval_ctx_bound :
     (* | _ => ctx_bound_st ub st' *)
     end.
 Proof.
-  intros. 
+  intros. rename H into H'. rename H0 into H0'.
   induction EVAL; try destruct v as [x' e' C_lam'];
   destruct INIT as [A B].
   - rewrite <- STATE in *. split; eauto.
-    specialize (A (addr_x C x) x' e' C_lam' ACCESS). eauto.
+    specialize (A addr x' e' C_lam' ACCESS). eauto.
   - destruct st. split; eauto.
   - apply IHEVAL3. clear IHEVAL3.
     simpl in B. 
@@ -434,10 +255,10 @@ Proof.
     simpl. unfold update_m. intros.
     destruct arg as [x'' e'' C_lam''].
     destruct IHEVAL2 as [A'' B''].
-    destruct (eq_p addr (t :: dy_level C_lam)); eauto.
+    destruct (eqb addr t); eauto.
     simpl in INvl. destruct INvl.
     inversion H; subst. simpl in B''. eauto.
-    simpl in A''. specialize (A'' (t :: dy_level C_lam) x0 e0 C_v H). eauto.
+    simpl in A''. specialize (A'' t x0 e0 C_v H). eauto.
   - apply IHEVAL2. clear IHEVAL2.
     simpl in B.
     assert (forall sC : st_ctx, In sC (snd (collect_ctx (dy_to_st C) m)) -> In sC ub).
@@ -476,10 +297,10 @@ Proof.
          simpl in B; intros; apply B; rewrite in_app_iff; right; 
          eauto).
     simpl. unfold update_m. intros.
-    destruct (eq_p addr (t :: dy_level C)); eauto.
+    destruct (eqb addr t); eauto.
     simpl in INvl. destruct INvl.
     inversion H; subst. simpl in B'. eauto.
-    simpl in A'. specialize (A' (t :: dy_level C) x0 e0 C_v H). eauto.
+    simpl in A'. specialize (A' t x0 e0 C_v H). eauto.
   - apply IHEVAL2. clear IHEVAL2.
     simpl in B. 
     assert (forall sC : st_ctx, In sC (snd (collect_ctx (dy_to_st C) m')) -> In sC ub).
@@ -501,15 +322,15 @@ Proof.
 Qed.
 
 Lemma reach_ctx_bound :
-  forall ub
-         C st e
+  forall `{Time T} ub
+         (C : @dy_ctx T) st e
          C' st' e'
          (INIT : ctx_bound_tm ub C st e)
          (REACH : <| C st e ~#> C' st' e' |>),
     ctx_bound_tm ub C' st' e'.
 Proof.
-  intros. induction REACH; eauto; 
-          apply IHREACH; destruct INIT as [A B].
+  intros. rename H into H'. rename H0 into H0'.
+  induction REACH; eauto; apply IHREACH; destruct INIT as [A B].
   - simpl in B. split; eauto.
     destruct (collect_ctx (dy_to_st C) e1).
     intros; apply B. simpl in *. rewrite in_app_iff. left; eauto.
@@ -525,10 +346,10 @@ Proof.
     apply eval_ctx_bound with (ub := ub) in ARG. destruct arg as [x'' e'' C''].
     destruct FN as [A' B']. destruct ARG as [A'' B''].
     split. simpl. unfold update_m. intros.
-    destruct (eq_p addr (t :: dy_level C_lam)).
+    destruct (eqb addr t).
     simpl in INvl. destruct INvl.
     inversion H; subst. simpl in B''. eauto.
-    simpl in A''. specialize (A'' (t :: dy_level C_lam) x0 e0 C_v H). eauto.
+    simpl in A''. specialize (A'' t x0 e0 C_v H). eauto.
     simpl in A''. specialize (A'' addr x0 e0 C_v INvl). eauto.
     rewrite dy_to_st_plugin. simpl. simpl in B'.
     destruct (collect_ctx (dy_to_st C_lam [[|st_c_lam x ([[||]])|]]) e).
@@ -563,10 +384,10 @@ Proof.
   - apply eval_ctx_bound with (ub := ub) in EVALx. destruct v as [x'' e'' C_lam''].
     destruct EVALx as [A' B'].
     split. simpl. unfold update_m. intros.
-    destruct (eq_p addr (t :: dy_level C)).
+    destruct (eqb addr t).
     simpl in INvl. destruct INvl.
     inversion H; subst. simpl in B'. eauto.
-    simpl in A'. specialize (A' (t :: dy_level C) x0 e0 C_v H). eauto.
+    simpl in A'. specialize (A' t x0 e0 C_v H). eauto.
     simpl in A'. specialize (A' addr x0 e0 C_v INvl). eauto.
     simpl in B. rewrite dy_to_st_plugin. simpl.
     destruct (collect_ctx (dy_to_st C [[|st_c_lete x ([[||]])|]]) m).
@@ -596,14 +417,14 @@ Proof.
 Qed.
 
 Theorem expr_ctx_bound :
-  forall e C' st' e'
-         (REACH : <| ([#||#]) (ST empty_mem true) e ~#> C' st' e' |>),
+  forall `{Time T} init e C' st' e'
+         (REACH : <| ([||]) (ST empty_mem init) e ~#> C' st' e' |>),
          In (dy_to_st C') (snd (collect_ctx ([[||]]) e)).
 Proof.
-  intros.
-  pose proof (reach_ctx_bound (snd (collect_ctx st_c_hole e)) ([#||#]) (ST empty_mem true) e C' st' e') as H.
+  intros. rename H into H'. rename H0 into H0'.
+  pose proof (reach_ctx_bound (snd (collect_ctx st_c_hole e)) ([||]) (ST empty_mem init) e C' st' e') as H.
   assert (ctx_bound_tm (snd (collect_ctx ([[||]]) e)) 
-                       ([#||#]) (ST empty_mem true) e) as FINAL.
+                       ([||]) (ST empty_mem init) e) as FINAL.
   - split; simpl; eauto. intros. inversion INvl. 
     destruct (collect_ctx ([[||]]) e); eauto.
   - apply H in FINAL; try apply REACH. 
